\documentclass[12pt]{article}
\usepackage[paper=letterpaper,margin=2cm]{geometry}

\usepackage{mathtools, amssymb, amsthm}
\usepackage{graphicx}
\usepackage{titling}
\usepackage{polynom}
\usepackage[table,xcdraw]{xcolor}
\usepackage{fancyhdr}
\usepackage{lipsum}
	
\pagestyle{fancy}
\fancyhf{}
\rhead{\small {Â© 2022 All Rights Reserved, Aiden Rosenberg}}
\rfoot{Page \thepage}

\setlength{\droptitle}{-6em}

\title{AP Classroom Problems Unit 1}
\author{Aiden Rosenberg}
\date{September 2022}

\begin{document}
\maketitle
\section{Thinking Backwards \& Substitution}
\begin{enumerate}
\item $$ \text{If } \int_{0}^{k} \frac{x}{x^2+4} \,dx=\frac{1}{2}\ln4 \text{, where } k>0 \text{, then } k=$$
\begin{enumerate}
    \item $u=x^2+4 \Longrightarrow \frac{du}{2x}= dx$
    \item $\int_{0}^{k} \frac{x}{x^2+4} \,dx$
$$\Longrightarrow \frac{1}{2} \int \frac{1}{u} \,du = \frac{1}{2}\ln|u|+C = \frac{1}{2} \ln|x^2+4| +C$$
$$\Longrightarrow \frac{1}{2} \ln|x^2+4| \bigg\rvert^{k}_{0}= \frac{1}{2}\ln|k^2+4|-\frac{1}{2}\ln(4)=\frac{1}{2}\ln4$$
$$\Longrightarrow \ln(\frac{k^2+4}{4})= \ln4$$
$$\Longrightarrow k^2+4 = 16 $$
$$\Longrightarrow k=\sqrt{12}$$
\end{enumerate}

\item $$ \int (e^x +e) \,dx$$
$$= e^x+ex +C$$

\item $$ \int (\sec(x)\cdot \tan(x) \,dx$$
$$= \sec(x)+C$$

\item $$\int_{0}^{3} (x+1)^{\frac{1}{2}} \,dx $$
\begin{enumerate}
    \item $u=x+1 \Longrightarrow du=dx$
\end{enumerate}
$$\Longrightarrow \int u^{\frac{1}{2}} \, du$$
$$\Longrightarrow \frac{2x^{\frac{3}{2}}}{3} \bigg\rvert^{0}_{3} = \frac{2(4)^{3/2}-2}{3}=\frac{14}{3}$$

\newpage
\item $$ \int \frac{x}{x^2-4} \,dx$$
\begin{enumerate}
    \item $u=x^2-4 \Longrightarrow \frac{du}{2x}=dx$
\end{enumerate}
$$\Longrightarrow \frac{1}{2} \int \frac{1}{u} \, du = \frac{1}{2}\ln|u| +C $$ 
$$\Longrightarrow \frac{1}{2}|x^2-4|+C$$

\item $$\int_{2}^{4} \frac{1}{5-3x} \,dx $$
$$= \frac{\ln|-3x+5|}{-3}$$
\begin{enumerate}
    \item $\int \frac{1}{ax+b} \, dx = \frac{\ln|ax+b|}{b}$
\end{enumerate}

\item $$ \int_{0}^{1} (x^3+x)(x^4+2x^2+9)^{1/2} \, dx$$ 
\begin{enumerate}
    \item $u=x^4+2x^2+9 \Longrightarrow du = (4x^3+4x)dx = 4(x^3+x)dx$
\end{enumerate}
$$\Longrightarrow \frac{1}{4}\int u^{1/2} \, du = \frac{u^{3/2}}{6}$$
$$\Longrightarrow \frac{(x^4+2x^2+9)^{3/2}}{6}\bigg\rvert_{0}^{1}$$
$$\Longrightarrow \frac{(12)^{3/2}-9^{3/2}}{6} = \frac{24\sqrt{3}-27}{6} = 4\sqrt{3}-\frac{9}{2}$$

\item $$\int_{\pi/6}^{\pi/2} (\sin^5(2x)\cdot \cos(2x)) \, dx$$
\begin{enumerate}
    \item $u=\sin(2x) \Longrightarrow du=2\cos(x) \, dx$
    \item $\sin(\pi)=0 \text{ \& } \sin(\pi/3)=\frac{\sqrt{3}}{2}$ 
    
    
\end{enumerate}
$$ \Longrightarrow\frac{1}{2}\int_{\frac{\sqrt{3}}{2}}^{0} u^5 \, du = \frac{-9}{256}$$

\item $$ \text{If } \int_{1}^{2} f(x-c) \, dx=5 \text { where $c$ is a constant, then}\int_{1-c}^{2-c} f(x) \, dx =5$$
\begin{enumerate}
    \item $u=x-c \Longrightarrow dx=du$ 
    \item $u_a = 1-c$ and $u_b=2-c$ \textit{Changing the bounds}
\end{enumerate}


\item $$\int \cos(3x)\, dx$$

\begin{enumerate}
    \item $u=3x \Longrightarrow \frac{du}{3}=dx$
\end{enumerate}
$$\Longrightarrow \frac{1}{3}\int \cos(u) \, du = \frac{1}{3}\sin(u) +C= \frac{1}{3}\sin(3x) +C$$
\end{enumerate}
\section{Integration by Parts, Substitution, and Anti-derivatives}
\begin{enumerate}
    \item $$\text{Let $g$ be a differentiable function such that } \int g(x)e^{\frac{x}{4}} \, dx = 4g(x)e^{\frac{x}{4}}-\int 8x^2e^{\frac{x}{4}} \, dx.$$ $$\\ \text{Which of the following could be an expression for $g(x)$? } $$
\begin{enumerate}
    \item $$\int g(x) \cdot h'(x) \, dx = g(x) \cdot h(x)-\int g'(x)\cdot h(x) \,dx$$
    \item $h'(x)=e^{\frac{x}{4}} \Longrightarrow h(x)=4e^{\frac{x}{4}}$
    \item $g'(x)=2x^2 \Longrightarrow g(x) = \frac{2x^3}{3}$
\end{enumerate}
    \item $$\int_{1}^{2}(9x^2-4x+1) \cdot \ln x \, dx$$
\begin{enumerate}
    \item Let $u=\ln(x) \Longrightarrow du=\frac{1}{x} dx$ 
    \item $dv=(9x^2-4x+1) dx \Longrightarrow  v= 3x^3 -2x^2+x$
\end{enumerate}
$$\Longrightarrow \ln(x)(3x^3-2x^2+x)-\int (3x^2-2x+1) \, dx$$
$$\Longrightarrow \ln(x)(3x^3-2x^2+x)-(x^3-x^2+x)$$
$$\Longrightarrow \ln(x)(3x^3-2x^2+x)-x^3+x^2-x) \bigg\rvert^{2}_{1}$$
$$\Longrightarrow \bigg(\ln(2)(3(8)-8+2)-8+4-2) \bigg) - \bigg(\ln(1)(3-2+1)-1+1-1 \bigg)$$
$$\Longrightarrow (18\ln(2)-6)  -(2\ln(1)-1)$$
$$\Longrightarrow 18\ln(2)-5$$
\item 
\begin{table}[h]
\begin{centering}

\begin{tabular}{lllll}
$x$ & $1$ & $2$ & $3$ & $4$ \\ \hline
\multicolumn{1}{l|}{$f(x)$} & $-2$ & $1$ & $6$ & $3$ \\
\multicolumn{1}{l|}{$f'(x)$} & $2$ & $4$ & $-1$ & $-4$
\end{tabular}

\end{centering}
\end{table}
The function $f$ has a continuous second derivative. The table above gives values of $f$ and its derivative, $f'$, at selected values of $x$. What is the value of $\int x \cdot f''(x) \, dx$ ?
\begin{enumerate}
    \item Let $u=x \Longrightarrow dx=du$
    \item $dv=f''(x) dx \Longrightarrow v=f'(x)$
\end{enumerate}

$$\Longrightarrow xf'(x)-\int f'(x) \, dx $$
$$ \Longrightarrow xf'(x)-f(x) \, dx \bigg\rvert^{2}_{1} $$
$$ \Longrightarrow \bigg( 2f'(2)-f(2) \bigg) - \bigg(f'(1)-f(1) \bigg) $$
$$ \Longrightarrow ((2)(4)-1)-(2--2)=7-4=3 $$


\item $$\int \frac{4x^4+3}{4x^5+15x+2} \, dx$$
\begin{enumerate}
    \item $u=4x^5+15x+2 \Longrightarrow du = (20x^4+15x)dx= 5(4x^4+3)dx$
\end{enumerate}
$$\Longrightarrow \frac{1}{5} \int \frac{1}{u} \, du$$
$$\Longrightarrow \frac{1}{5} \ln|u|+C$$
$$\Longrightarrow \frac{1}{5} \ln|4x^5+15x+2| + C$$

\item $$\int_{0}^{1} (x+2)(3x^2+12x+1)^{1/2} \, dx$$
\begin{enumerate}
    \item Let $u=3x^2+12x+1 \Longrightarrow du=6(x+2)dx$
    \item $b=3(1)^2+12+12=16$ \& $a=3(0)+12(0)+1=1$
\end{enumerate}
$$\Longrightarrow \frac{1}{6}\int_{1}^{16} u^{1/2} \, du $$
$$\Longrightarrow \frac{1}{6} \cdot \frac{2u^{3/2}}{3} \bigg\rvert^{16}_{1}$$
$$\Longrightarrow\frac{u^{3/2}}{9} \bigg\rvert^{16}_{1} = \frac{64-1}{9}=7$$

\item $$\int \frac{1}{x^2+4} \, dx$$
$$\Longrightarrow \frac{1}{4}\int \frac{1}{(\frac{x^2}{4}+1)} \, dx$$
\begin{enumerate}
    \item Let $u^2=\frac{x^2}{4} \Longrightarrow u=\frac{x}{2} \Longrightarrow 2du=dx$
\end{enumerate}
$$\Longrightarrow \frac{1}{2} \int \frac{1}{u^2+1} \, du$$
$$\Longrightarrow \frac{1}{2}\arctan(u)+C $$
$$\Longrightarrow \frac{1}{2}\arctan(\frac{x}{2})+C $$

\item $$\int \frac{3x^2+4x+1}{3x^3+6x^2+3x+5} \, dx$$
\begin{enumerate}
    \item Let $u=3x^3+6x^2+3x+5 \Longrightarrow du=3(3x^2+4x+1)dx$
\end{enumerate}
$$\Longrightarrow \frac{1}{3} \int \frac{1}{u} \, du$$
$$\Longrightarrow \frac{1}{3} \ln|u|+C$$
$$\Longrightarrow \frac{1}{3} \ln|3x^3+6x^2+3x+5|+C$$

\item $$\int \frac{1}{\sqrt{9-x^2}} \, dx$$
$$\Longrightarrow \int \frac{1}{\sqrt{9(1-\frac{x^2}{9})}}$$
$$\Longrightarrow \frac{1}{3}\int \frac{1}{\sqrt{(1-\frac{x^2}{9})}}$$
\begin{enumerate}
    \item Let $u^2=\frac{x^2}{9} \Longrightarrow u=\frac{x}{3} \Longrightarrow 3du=dx$
\end{enumerate}
$$\Longrightarrow \int \frac{1}{\sqrt{1-u^2}} \,du$$
$$\Longrightarrow \arcsin(u) +C$$
$$\Longrightarrow \arcsin(\frac{x}{3}) +C$$

\item See \#7 in section 1
\end{enumerate}

\section{All anti-differentiation strategies in one assignment.}
\begin{enumerate}
   
\item $$\int_{0}^{1} x \sqrt{1+8x^2} \, dx $$
\begin{enumerate}
    \item Let $u=1+8x^2 \Longrightarrow \frac{du}{16} = x \cdot dx $
    \item $b = 1 + 8(1)^2 = 9$
    \item $a = 1+8(0)^2=1$
\end{enumerate}

$$\Longrightarrow \frac{1}{16} \int_{1}^{9} u^{1/2} \, du = \frac{1}{16} \cdot \frac{2u^{3/2}}{3} \bigg\rvert^{1}_{9} $$
$$ \Longrightarrow \frac{u^{3/2}}{24} \bigg\rvert^{1}_{9} = \frac{27}{24}-\frac{1}{24} =\frac{26}{24} =\frac{13}{12}$$

\item  $$\int_{0}^{1} \frac{5x+8}{x^2+3x+2} \, dx$$
$$\Longrightarrow  \frac{5x+8}{(x+2)(x+1)}$$
$$\Longrightarrow \frac{A}{x+1} +\frac{B}{x+2}$$
$$\Longrightarrow \frac{A(x+2)+B(x+1)}{(x+2)(x+1)}=   \frac{5x+8}{(x+2)(x+1)}$$
$$\Longrightarrow A+B=5 \quad \& \quad 2A+B=8$$
$$\Longrightarrow A=3 \quad \& \quad B=2 $$
$$\Longrightarrow \int \frac{3}{x+1} +\frac{2}{x+2} \, dx$$
$$\Longrightarrow \bigg[3\ln(x+1)+2\ln(x+2)\bigg]^{1}_{0}$$
$$\Longrightarrow \bigg(3 \ln(2)+2\ln(3) \bigg) - \bigg(3 \ln(1)+2\ln(2) \bigg)$$
$$\Longrightarrow 18 $$



\item If $f$ is a function such that $f'(x)=-f(x)$, then $\int xf(x) \,dx =$
\begin{enumerate}
    \item Let $u=x \Longrightarrow du=dx$
    \item $dv=f(x) \,dx \Longrightarrow v=\int f(x) \, dx = -\int f'(x) \,dx = -f(x)$
\end{enumerate}
$$-x \cdot f(x)-\int -f'(x) \, dx$$
$$-x \cdot f(x)+\int f'(x) \, dx$$
$$-x \cdot f(x)+f(x) +C $$
$$(1-x)\cdot f(x) +C $$
$$-f(x)\cdot(x+1) +C $$
\item See \#9 in section 1

\item $$\int \frac{-2x^2+7x-8}{(x+2)(2x-1)(1-x)} \, dx$$
$$\Longrightarrow \frac{A}{x+2} + \frac{B}{2x-1} +\frac{C}{1-x}$$
$$\Longrightarrow \frac{A(2x-1)(1-x)+B(x+2)(1-x)+C(x+2)(2x-1)}{(x+2)(2x-1)(1-x)} = \frac{-2x^2+7x-8}{(x+2)(2x-1)(1-x)}$$

\[   \left\{
\begin{array}{lll}
    -2A-B+2C &=-2 \\
    3A-B+3C &=7 \\
    -A+2B-2C&=-8 \\
\end{array} 
\right. \]
$$\Longrightarrow A=2 \quad  B=-4 \quad C=-1$$
$$\Longrightarrow \int \bigg( \frac{2}{x+2} + \frac{-4}{2x-1} +\frac{-1}{1-x} \bigg) \, dx$$
$$\Longrightarrow 2\ln|x+2|-2\ln|2x-1|+\ln|1-x| +C$$
\item $$\int (x^3+1)^2 \, dx$$
\begin{enumerate}
    \item $(x^3+1)^2 = x^6+2x^3+1$
\end{enumerate}
$$\Longrightarrow \int (x^6+2x^3+1) \, dx$$
$$\Longrightarrow \frac{1}{7}x^7 +\frac{1}{2}x^4 +x +C$$

\item $$\int \sqrt{x} \bigg(9x^3-2\sqrt{x}+\frac{8}{x}\bigg) \, dx$$
$$\Longrightarrow \int (9x^{7/2}-2x+\frac{8}{x^{1/2}})$$
$$\Longrightarrow 2x^{9/2} -x^2 +16x^{1/2} +C$$

\item $$\int_{0}^{5} \frac{3x+11}{x+2} \, dx$$
\begin{enumerate}
    \item \polylongdiv{3x+11}{x+2} $$\Longrightarrow \int_{0}^{5} 3+ \frac{5}{x+2} \, dx$$
    $$\Longrightarrow 3x+5\ln(x+2)\bigg\rvert_{0}^{5} =5\ln(\frac{7}{2})+15$$
    \item Let $u=x+2 \Longrightarrow du = dx$
    $$ \int_{2}^{7} 3 + \frac{5}{u} \, du = 3u +5\ln(u) \bigg\rvert_{2}^{7} = 5\ln(\frac{7}{2})+15  $$
\end{enumerate}


\item $$\int \frac{4}{x^2+4x+8} \, dx$$
$$\Longrightarrow 4\int \frac{1}{x^2+4x+8} \, dx$$
$$\Longrightarrow 4\int \frac{1}{(x+2)^2 + 4} \, dx$$
$$\Longrightarrow \int \frac{1}{\frac{(x+2)^2}{4} + 1} \, dx$$
\begin{enumerate}
    \item Let $u^2=\frac{(x+2)^2}{4} \Longrightarrow u= \frac{x+2}{2}= \frac{x}{2}+1$
    \item $\Longrightarrow 2du=dx$
\end{enumerate}
$$\Longrightarrow 2\int \frac{1}{u^2+1} \, du$$
$$\Longrightarrow 2\arctan (u) + C$$
$$\Longrightarrow 2\arctan (\frac{x+2}{2}) + C$$

\item $$\int \frac{1}{x^2-2x+2} \, dx$$
$$\Longrightarrow \int \frac{1}{(x-1)^2+1} \, dx$$
\begin{enumerate}
    \item Let $u=x-1 \Longrightarrow du=dx$
\end{enumerate}
$$\Longrightarrow  \int \frac{1}{u^2+1} \, dx$$
$$\Longrightarrow  \arctan(u) + C$$
$$\Longrightarrow  \arctan(x-1) + C$$

\item $$\int \bigg(5e^{2x}+\frac{1}{x}\bigg) \, dx$$
\begin{enumerate}
    \item Let $u=2x \Longrightarrow \frac{du}{2}=dx$
\end{enumerate}
$$\Longrightarrow \frac{5}{2}\int e^{u} \, du+ \int \frac{1}{x} \, dx$$
$$\Longrightarrow \frac{5}{2}e^{2x} + \ln|x| +C$$

\item See \#2 in section 2

\item $$ \text{Using the substitution $u=\sqrt{x}$, find an equivalent form of }\int_{1}^{4} \frac{e^{\sqrt{x}}}{\sqrt{x}} \, dx$$  
\begin{enumerate}
    \item If $u=\sqrt{x} \Longrightarrow 2du=\frac{1}{\sqrt{x}}$
    \item $b=\sqrt{4} = 2$ \& $a=\sqrt{1} = 1$
\end{enumerate}
$$\Longrightarrow 2\int_{1}^{2} e^u \, du = 2e(e-1)$$

 \item 

\begin{table}[h]
\begin{center}

\begin{tabular}{l|ll}
$x$ & $2$ & $4$ \\ \hline
$f(x)$ & $7$ & $13$ \\
$g(x)$ & $2$ & $9$ \\
$g'(x)$ & $1$ & $7$ \\
$g''(x)$ & $5$ & $8$
\end{tabular}
\end{center}
\end{table}
The table above gives selected values of twice-differentiable functions $f$ and $g$, as well as the first two derivatives of $g$. If $f'(x)=3$ for all values of $x$, what is the value of $\int_{2}^{4} f(x)\cdot g''(x) \, dx$?
\begin{enumerate}
    \item Let $u=f(x) \Longrightarrow f'(x)dx$
    \item $dv=g''(x)dx \Longrightarrow v=g'(x)$
\end{enumerate}
$$\Longrightarrow f(x)\cdot g'(x)-\int g'(x)\cdot f'(x) \, dx$$
$$\Longrightarrow f(x)\cdot g'(x)-3\int g'(x)$$
$$\Longrightarrow f(x)\cdot g'(x)-3g(x) \bigg\rvert_{2}^{4}$$
$$\bigg (f(4)\cdot g'(4)-3g(4) \bigg) - \bigg (f(2) \cdot g'(2)\cdot 3g(2) \bigg)$$
$$\bigg (13\cdot 7-3(9) \bigg) - \bigg (7 \cdot - 1\cdot 6 \bigg) = 63$$

\item $$\text{The function $f$ is continuous and}\int_{0}^{8} f(u)\,du=6 \text{. What is the value of}\int_{1}^{3} x \cdot f(x^2-1)\,dx \text{?}$$
\begin{enumerate}
    \item Let $u=x^2-1 \Longrightarrow du=2xdx$ 
\end{enumerate}
$$\Longrightarrow \frac{1}{2} \int^{8}_{0} f(u) \, du = 3$$
\end{enumerate}


\end{document}


